weaken conditions on sent_packets

ironfleet/src/Dafny/Distributed/Protocol/RSL/FailureProof/Common/definitions.i.dfy
@@ -73,4 +73,21 @@ function Get2bCount(s:LReplica, opn:OperationNumber, ballot:Ballot) : int
 }
 
 
+predicate IsUndelivered_1aPkt(ts:TimestampedRslState, p:TimestampedRslPacket) {
+  p !in ts.undeliveredPackets && p.msg.v.RslMessage_1a?
+}
+
+predicate IsUndelivered_1bPkt(ts:TimestampedRslState, p:TimestampedRslPacket) {
+  p !in ts.undeliveredPackets && p.msg.v.RslMessage_1b?
+}
+
+predicate IsUndelivered_2aPkt(ts:TimestampedRslState, p:TimestampedRslPacket) {
+  p !in ts.undeliveredPackets && p.msg.v.RslMessage_2a?
+}
+
+predicate IsUndelivered_2bPkt(ts:TimestampedRslState, p:TimestampedRslPacket) {
+  p !in ts.undeliveredPackets && p.msg.v.RslMessage_2b?
+}
+
+
 }
